theories/hoare.v
@@ -5,6 +5,7 @@ Require Import Regex2NFA.theories.regex.
 Require Import Coq.ZArith.ZArith.
 From StateMonad.monaderror Require Import monadEbasic monadEwhile monadesafe_lib monadEhoare.
 
+Import MonadwitherrDeno.
 Import MonadNotation.
 Local Open Scope stmonad_scope.
 Local Open Scope Z_scope.
@@ -21,11 +22,12 @@ Lemma st_nograph_inc {T: Type} :
                       (forall n, g.(vvalid) n -> v < n <= s2.(max_v)) /\
                       (forall n, g.(evalid) n -> e < n <= s2.(max_e)) /\
                       forall str, exp_match r str <->
-                                  G_match_string G el.(startVertex) el.(endVertex) str
+                                  G_match_str G el.(startVertex) el.(endVertex) str
         ).
 Proof.
 Admitted.
 
+(** low_level prop *)
 Lemma st_graph_inc {T: Type} :
   forall (r : reg_exp T), exists (v e : Z) (G: @pg_nfa T),
   Hoare (fun s1 => s1.(max_v') = v /\
@@ -37,44 +39,42 @@ Lemma st_graph_inc {T: Type} :
                       s2.(max_e') > e /\
                       (forall n, g.(vvalid) n -> n <= s2.(max_v')) /\
                       (forall n, g.(evalid) n -> n <= s2.(max_e'))
-                      (** TODO: safeExec *)
         ).
 Proof.
 Admitted.
 
-(** high_level (st_nograph)
-(v, e)
-(sv, ev, G_ret) <- execute
-(v', e')
-*)
-(** low_level (st_graph)
-(v, e, G)
-(sv, ev) <- execute'
-(v', e', G')
-*)
-(* Lemma graph_corr_prop {T: Type} :
-  forall (G: @pg_nfa T) (r: reg_exp T) (v e: Z),
-  exists (G_ret: @pg_nfa T) (v' e' sv ev : Z),
-  (** low_level : @Hoare state' elem' *)
-  Hoare (fun s1 => s1.(st_graph) = G /\
-                   s1.(max_v') = v /\
-                   s1.(max_e') = e )
-        (regexToNFA' r)
-        (fun el s2 => s2.(max_v') = v' /\
-                      s2.(max_e') = e' /\
-                      G1_union G G_ret s2.(st_graph) ) /\
-  (** high_level : @Hoare state elem *)
-  Hoare (fun s1 => s1.(max_v) = v /\
-                   s1.(max_e) = e)
-        (regexToNFA r)
-        (fun el s2 => s2.(max_v) = v' /\
-                      s2.(max_e) = e' /\
-                      el.(startVertex) = sv /\
-                      el.(endVertex) = ev /\
-                      el.(graph) = G_ret).
-  (* v' >= v /\ e' >= e *)
-  (* sv > v /\ sv <= v' /\ ev > v /\ ev <= v' *)
-  (** el.(graph) rel *)
-  (*? edge rel *)
+Lemma st_graph_refine {T: Type} :
+  (** ∀ X, *)
+  forall (r : reg_exp T) (G: @pg_nfa T) X,
+  Hoare ( fun s1 =>
+            (** safeExec_X P_abs c_abs X *)
+            (safeExec (fun s => s.(max_v) = s1.(max_v') /\ s.(max_e) = s1.(max_e'))
+                      (regexToNFA r)
+                      X) /\
+            (*** P_con *)
+            s1.(st_graph) = G
+            (** G \forall v e, <= max_v max_e *)
+        )
+        (regexToNFA' r) (** c_con *)
+        ( 
+          fun el' s2 =>
+            (** ∃ a, safeExec_X Q_abs(a) skip *)
+            exists el, (safeExec (
+                                   fun s => s.(max_v) = s2.(max_v') /\
+                                            s.(max_e) = s2.(max_e')
+                                 )
+                                 (return el) (*? skip *)
+                                 X
+                       ) /\
+            (** Q_con(a) *)
+            let g := G.(pg) in
+              el'.(startVertex') = el.(startVertex) /\
+              el'.(endVertex') = el.(endVertex) /\
+              G_union_rel G el.(graph) s2.(st_graph) (** refinement *)
+        ).
 Proof.
-Admitted. *)
+Admitted.
+
+Check safeExec.
+
+
